non_constructive.v
@@ -1,0 +1,30 @@
+From Casper
+Require Import vlsm_preamble.
+
+Axiom proof_irrelevance : forall (P : Prop) (p1 p2 : P), p1 = p2.
+
+Lemma exist_eq
+  {X}
+  (P : X -> Prop)
+  (a b : {x : X | P x})
+  : a = b <-> proj1_sig a = proj1_sig b.
+Proof.
+  destruct a as [a Ha]; destruct b as [b Hb]; simpl.
+  split; intros Heq.
+  - inversion Heq. reflexivity.
+  - subst. apply f_equal. apply proof_irrelevance.
+Qed.
+
+Lemma DepEqDec
+  {X}
+  (Heqd : EqDec X)
+  (P : X -> Prop)
+  : EqDec {x : X | P x}.
+Proof.
+  intros [x Hx] [y Hy].
+  specialize (Heqd x y).
+  destruct Heqd as [Heq | Hneq].
+  - left. subst. apply f_equal. apply proof_irrelevance.
+  - right.  intros Heq. apply Hneq. inversion Heq. reflexivity.
+Qed.
+
