vlsm_preamble.v
@@ -1,0 +1,15 @@
+
+Class EqDec X :=
+  eq_dec : forall x y : X, {x = y} + {x <> y}.
+
+
+Lemma nat_eq_dec : EqDec nat.
+Proof.
+  unfold EqDec. induction x; destruct y.
+  - left. reflexivity.
+  - right. intros C; inversion C.
+  - right. intros C; inversion C.
+  - specialize (IHx y). destruct IHx as [Heq | Hneq].
+    + left. subst. reflexivity.
+    + right. intros Heq. inversion Heq. contradiction.
+Qed.
